double_normalize_type for well formed types in well formed envs.

src/coq/TypeUtil.v
@@ -4,6 +4,8 @@ Require Import Vellvm.LLVMAst.
 Require Import Vellvm.AstLib.
 Require Import Vellvm.Classes.
 Require Import Coqlib.
+Require Import Coq.Logic.FunctionalExtensionality.
+
 
 Import ListNotations.
 Open Scope list_scope.
@@ -184,6 +186,12 @@ Inductive guarded_typ : ident -> list (ident * typ) -> typ -> Prop :=
     forall (id : ident) (env : list (ident * typ)),
       guarded_typ id env TYPE_X86_mmx
 
+| guarded_typ_Function :
+    forall (id : ident) (env : list (ident * typ)) (ret : typ) (args : list typ),
+      guarded_typ id env ret ->
+      (forall a, In a args -> guarded_typ id env a) ->
+      guarded_typ id env (TYPE_Function ret args)
+
 | guarded_typ_Array :
     forall (id : ident) (env : list (ident * typ)) (sz : int) (t : typ),
       guarded_typ id env t -> guarded_typ id env (TYPE_Array sz t)
@@ -196,7 +204,7 @@ Inductive guarded_typ : ident -> list (ident * typ) -> typ -> Prop :=
 | guarded_typ_Packed_struct :
     forall (id : ident) (env : list (ident * typ)) (t : typ) (fields : list typ),
       (forall f, In f fields -> guarded_typ id env f) ->
-      guarded_typ id env (TYPE_Struct fields)
+      guarded_typ id env (TYPE_Packed_struct fields)
 
 | guarded_typ_Opaque :
     forall (id : ident) (env : list (ident * typ)),
@@ -209,7 +217,7 @@ Inductive guarded_typ : ident -> list (ident * typ) -> typ -> Prop :=
 | guarded_typ_Identified_Some :
     forall (id : ident) (env : list (ident * typ)) (id' : ident) (t : typ),
       id <> id' ->
-      Some (id', t) = find (fun a => eqb_ident id' (fst a)) env ->
+      Some (id', t) = find (fun a => Ident.eq_dec id' (fst a)) env ->
       guarded_typ id env t ->
       guarded_typ id' env t ->
       guarded_typ id env (TYPE_Identified id')
@@ -217,10 +225,33 @@ Inductive guarded_typ : ident -> list (ident * typ) -> typ -> Prop :=
 | guarded_typ_Identified_None :
     forall (id : ident) (env : list (ident * typ)) (id' : ident),
       id <> id' ->
-      None = find (fun a => eqb_ident id' (fst a)) env ->
+      None = find (fun a => Ident.eq_dec id' (fst a)) env ->
       guarded_typ id env (TYPE_Identified id')
 .
 
+
+Inductive first_class_typ : typ -> Prop :=
+| first_class_I : forall sz, first_class_typ (TYPE_I sz)
+| first_class_Pointer : forall t, first_class_typ (TYPE_Pointer t)
+| first_class_Void : first_class_typ TYPE_Void
+| first_class_Half : first_class_typ TYPE_Half
+| first_class_Float : first_class_typ TYPE_Float
+| first_class_Double : first_class_typ TYPE_Double
+| first_class_X86_fp80 : first_class_typ TYPE_X86_fp80
+| first_class_Fp128 : first_class_typ TYPE_Fp128
+| first_class_Ppc_fp128 : first_class_typ TYPE_Ppc_fp128
+| first_class_Metadata : first_class_typ TYPE_Metadata
+| first_class_X86_mmx : first_class_typ TYPE_X86_mmx
+| first_class_Array : forall sz t, first_class_typ (TYPE_Array sz t)
+| first_class_Struct : forall fields, first_class_typ (TYPE_Struct fields)
+| first_class_Packed_struct : forall fields, first_class_typ (TYPE_Packed_struct fields)
+| first_class_Opaque : first_class_typ TYPE_Opaque
+| first_class_Vector : forall sz t, first_class_typ (TYPE_Vector sz t)
+| first_class_Identified : forall id, first_class_typ (TYPE_Identified id)
+.
+
+Definition function_ret_typ (t : typ) : Prop :=
+  first_class_typ t /\ t <> TYPE_Metadata.
 
 (* Inductive predicate for well-formed LLVM types.
 
@@ -237,6 +268,8 @@ Inductive guarded_typ : ident -> list (ident * typ) -> typ -> Prop :=
    - Vectors of size 0
    - Arrays with unsized elements
    - Recursive structures (must be guarded by a pointer) *)
+
+
 Inductive wf_typ : list (ident * typ) -> typ -> Prop :=
 | wf_typ_Pointer:
     forall (defs : list (ident * typ)) (t : typ),
@@ -282,6 +315,14 @@ Inductive wf_typ : list (ident * typ) -> typ -> Prop :=
     forall (defs : list (ident * typ)),
       wf_typ defs TYPE_X86_mmx
 
+| wf_typ_Function :
+    forall (defs : list (ident * typ)) (ret : typ) (args : list typ),
+      function_ret_typ ret ->
+      wf_typ defs ret ->
+      (forall (a : typ), In a args -> sized_typ defs a) ->
+      (forall (a : typ), In a args -> wf_typ defs a) ->
+      wf_typ defs (TYPE_Function ret args)
+
 (* Arrays are only well formed if the size is >= 0, and the element type is sized. *)
 | wf_typ_Array :
     forall (defs : list (ident * typ)) (sz : int) (t : typ),
@@ -298,18 +339,22 @@ Inductive wf_typ : list (ident * typ) -> typ -> Prop :=
    that it refers to *unless* it is guarded by a pointer. *)
 | wf_typ_Identified :
     forall (defs : list (ident * typ)) (id : ident),
-      (exists (t : typ), In (id, t) defs -> guarded_typ id defs t -> wf_typ defs t) ->
+      (exists t, In (id, t) defs) ->
+      (forall (t : typ), In (id, t) defs -> guarded_typ id defs t) ->
+      (forall (t : typ), In (id, t) defs -> wf_typ defs t) ->
       wf_typ defs (TYPE_Identified id)
 
 (* Fields of structure must be sized types *)
 | wf_typ_Struct :
     forall (defs : list (ident * typ)) (fields : list typ),
-      (forall (f : typ), In f fields -> sized_typ defs f -> wf_typ defs f) ->
+      (forall (f : typ), In f fields -> sized_typ defs f) ->
+      (forall (f : typ), In f fields -> wf_typ defs f) ->
       wf_typ defs (TYPE_Struct fields)
 
 | wf_typ_Packed_struct :
     forall (defs : list (ident * typ)) (fields : list typ),
-      (forall (f : typ), In f fields -> sized_typ defs f -> wf_typ defs f) ->
+      (forall (f : typ), In f fields -> sized_typ defs f) ->
+      (forall (f : typ), In f fields -> wf_typ defs f) ->
       wf_typ defs (TYPE_Packed_struct fields)
 
 | wf_typ_Opaque :
@@ -318,8 +363,117 @@ Inductive wf_typ : list (ident * typ) -> typ -> Prop :=
 .
 
 
+Hint Constructors wf_typ.
+
+
 Definition wf_env (env : list (ident * typ)) : Prop :=
-  NoDup (map fst env) -> Forall (wf_typ env) (map snd env).
+  NoDup (map fst env) /\ Forall (wf_typ env) (map snd env).
+
+
+Inductive guarded_wf_typ : list (ident * typ) -> typ -> Prop :=
+| guarded_wf_typ_Pointer:
+    forall (defs : list (ident * typ)) (t : typ),
+      guarded_wf_typ defs (TYPE_Pointer t)
+
+| guarded_wf_typ_I :
+    forall (defs : list (ident * typ)) (sz : int),
+      sz > 0 -> guarded_wf_typ defs (TYPE_I sz)
+
+| guarded_wf_typ_Void :
+    forall (defs : list (ident * typ)),
+      guarded_wf_typ defs TYPE_Void
+
+| guarded_wf_typ_Half :
+    forall (defs : list (ident * typ)),
+      guarded_wf_typ defs TYPE_Half
+
+| guarded_wf_typ_Float :
+    forall (defs : list (ident * typ)),
+      guarded_wf_typ defs TYPE_Float
+
+| guarded_wf_typ_Double :
+    forall (defs : list (ident * typ)),
+      guarded_wf_typ defs TYPE_Double
+
+| guarded_wf_typ_X86_fp80 :
+    forall (defs : list (ident * typ)),
+      guarded_wf_typ defs TYPE_X86_fp80
+
+| guarded_wf_typ_Fp128 :
+    forall (defs : list (ident * typ)),
+      guarded_wf_typ defs TYPE_Fp128
+
+| guarded_wf_typ_Ppc_fp128 :
+    forall (defs : list (ident * typ)),
+      guarded_wf_typ defs TYPE_Ppc_fp128
+
+| guarded_wf_typ_Metadata :
+    forall (defs : list (ident * typ)),
+      guarded_wf_typ defs TYPE_Metadata
+
+| guarded_wf_typ_X86_mmx :
+    forall (defs : list (ident * typ)),
+      guarded_wf_typ defs TYPE_X86_mmx
+
+| guarded_wf_typ_Function :
+    forall (defs : list (ident * typ)) (ret : typ) (args : list typ),
+      function_ret_typ ret ->
+      guarded_wf_typ defs ret ->
+      (forall (a : typ), In a args -> sized_typ defs a) ->
+      (forall (a : typ), In a args -> guarded_wf_typ defs a) ->
+      guarded_wf_typ defs (TYPE_Function ret args)
+
+(* Arrays are only well formed if the size is >= 0, and the element type is sized. *)
+| guarded_wf_typ_Array :
+    forall (defs : list (ident * typ)) (sz : int) (t : typ),
+      sz >= 0 -> sized_typ defs t -> guarded_wf_typ defs t -> guarded_wf_typ defs (TYPE_Array sz t)
+
+(* Vectors of size 0 are not allowed, and elemnts must be of element_typ. *)
+| guarded_wf_typ_Vector :
+    forall (defs : list (ident * typ)) (sz : int) (t : typ),
+      sz > 0 -> element_typ t -> guarded_wf_typ defs t -> guarded_wf_typ defs (TYPE_Vector sz t)
+
+(* This lax form doesn't care if the identifier is actually in the
+   typing environment.
+
+   Additionally the identifier must not occur anywhere in the type
+   that it refers to *unless* it is guarded by a pointer. *)
+| guarded_wf_typ_Identified :
+    forall (defs : list (ident * typ)) (id : ident),
+      (exists t, In (id, t) defs) ->
+      (forall (t : typ), In (id, t) defs -> guarded_typ id defs t) ->
+      (forall (t : typ), In (id, t) defs -> guarded_wf_typ defs t) ->
+      guarded_wf_typ defs (TYPE_Identified id)
+
+(* Fields of structure must be sized types *)
+| guarded_wf_typ_Struct :
+    forall (defs : list (ident * typ)) (fields : list typ),
+      (forall (f : typ), In f fields -> sized_typ defs f) ->
+      (forall (f : typ), In f fields -> guarded_wf_typ defs f) ->
+      guarded_wf_typ defs (TYPE_Struct fields)
+
+| guarded_wf_typ_Packed_struct :
+    forall (defs : list (ident * typ)) (fields : list typ),
+      (forall (f : typ), In f fields -> sized_typ defs f) ->
+      (forall (f : typ), In f fields -> guarded_wf_typ defs f) ->
+      guarded_wf_typ defs (TYPE_Packed_struct fields)
+
+| guarded_wf_typ_Opaque :
+    forall (defs : list (ident * typ)),
+      guarded_wf_typ defs TYPE_Opaque
+.
+
+Hint Constructors guarded_wf_typ.
+
+
+Theorem wf_typ_is_guarded_wf_typ :
+  forall env t,
+    wf_typ env t ->
+    guarded_wf_typ env t.
+Proof.
+  intros env t H.
+  induction H; auto.
+Qed.
 
 
 Inductive unrolled_typ : typ -> Prop :=
@@ -426,6 +580,32 @@ Qed.
 Hint Resolve wf_lt_typ_order.
 Hint Constructors lex_ord.
 
+Definition length_order {A : Type} (l1 l2 : list A) :=
+  (List.length l1 < List.length l2)%nat.
+
+
+Lemma lengthOrder_wf' : forall A len, forall ls, (List.length ls <= len)%nat -> Acc (@length_order A) ls.
+  unfold length_order; induction len.
+  - intros ls H. inversion H. rewrite length_zero_iff_nil in H1. subst.
+    constructor. intros y H0. inversion H0.
+  - intros ls H. inversion H.
+    + constructor. intros y H0. apply IHlen. omega.
+    + auto.
+Defined.
+
+Theorem lengthOrder_wf : forall A, well_founded (@length_order A).
+  red; intros A a; eapply lengthOrder_wf'; eauto.
+Defined.
+
+
+Theorem wf_length_typ_order :
+  forall A,
+    well_founded (lex_ord (@length_order A) typ_order).
+Proof.
+  intros A. apply wf_lex_ord.
+  apply lengthOrder_wf. apply wf_typ_order.
+Defined.
+
 
 Lemma map_In {A B : Type} (l : list A) (f : forall (x : A), In x l -> B) : list B.
 Proof.
@@ -434,7 +614,7 @@ Proof.
   - refine (f a _ :: IHl _).
     + simpl. auto.
     + intros x H. apply (f x). simpl. auto.
-Qed.
+Defined.
 
 
 Fixpoint remove_key {A B : Type} (eq_dec : (forall (x y : A), {x = y} + {x <> y})) (a : A) (l : list (A * B)) : list (A * B) :=
@@ -445,6 +625,13 @@ Fixpoint remove_key {A B : Type} (eq_dec : (forall (x y : A), {x = y} + {x <> y}
     | left _ => t
     | right _ => (h, b) :: remove_key eq_dec a t
     end
+  end.
+
+
+Fixpoint remove_keys {A B : Type} (eq_dec : (forall (x y : A), {x = y} + {x <> y})) (keys : list A) (l : list (A * B)) : list (A * B) :=
+  match keys with
+  | nil => l
+  | key :: rest_of_keys => remove_keys eq_dec rest_of_keys (remove_key eq_dec key l)
   end.
 
 
@@ -463,6 +650,61 @@ Proof.
       destruct H.
       * inversion H. subst. contradiction.
       * assumption.
+Qed.
+
+
+Lemma remove_key_not_in :
+  forall (A B : Type) (a : A) eq_dec (l : list (A * B)),
+    ~ In a (map fst l) ->
+    remove_key eq_dec a l = l.
+Proof.
+  induction l; intros H.
+  - reflexivity.
+  - simpl in *. destruct a0. destruct (eq_dec a a0).
+    + intuition.
+    + rewrite IHl; intuition.
+Qed.
+
+
+Lemma remove_key_commutes :
+  forall (A B : Type) (k1 k2 : A) eq_dec (l : list (A * B)),
+    remove_key eq_dec k1 (remove_key eq_dec k2 l) = remove_key eq_dec k2 (remove_key eq_dec k1 l).
+Proof.
+  intros A B k1 k2 eq_dec l.
+  induction l; auto.
+  simpl. destruct a.
+  destruct (eq_dec k2 a) eqn:Hk2a.
+  - destruct (eq_dec k1 a).
+    + subst; auto.
+    + subst. simpl. destruct (eq_dec a a); try contradiction.
+      reflexivity.
+  - destruct (eq_dec k1 a) eqn:Hk1a.
+    + subst. simpl. destruct (eq_dec a a); try contradiction.
+      reflexivity.
+    + simpl. rewrite Hk2a. rewrite Hk1a. rewrite IHl.
+      reflexivity.
+Qed.  
+
+
+Lemma remove_key_keys :
+  forall (A B : Type) (keys : list A) eq_dec (key : A) (l : list (A * B)),
+    remove_key eq_dec key (remove_keys eq_dec keys l) = remove_keys eq_dec (key :: keys) l.
+Proof.
+  intros A B keys.
+  induction keys; intros eq_dec key l; auto.
+  simpl in *.
+  rewrite IHkeys.
+  apply f_equal.
+  apply remove_key_commutes.
+Qed.
+
+
+Lemma remove_keys_key :
+  forall (A B : Type) (keys : list A) eq_dec (key : A) (l : list (A * B)),
+    remove_keys eq_dec keys (remove_key eq_dec key l) = remove_keys eq_dec (key :: keys) l.
+Proof.
+  intros A B keys.
+  induction keys; intros eq_dec key l; auto.
 Qed.
 
 
@@ -490,7 +732,7 @@ Program Fixpoint normalize_type (env : list (ident * typ)) (t : typ) {measure (L
     TYPE_Vector sz nt
 
   | TYPE_Identified id =>
-    match find (fun a => eqb_ident id (fst a)) env with
+    match find (fun a => Ident.eq_dec id (fst a)) env with
     | None => TYPE_Identified id
     | Some (_, t) => normalize_type (remove_key Ident.eq_dec id env) t
     end
@@ -512,6 +754,502 @@ Next Obligation.
   left.
   symmetry in Heq_anonymous. apply find_some in Heq_anonymous. destruct Heq_anonymous as [Hin Heqb_ident].
   simpl in Heqb_ident.
-  apply eqb_ident_correct in Heqb_ident. subst.
-  eapply remove_key_in. apply Hin.
+  destruct (Ident.eq_dec id wildcard'). subst. eapply remove_key_in. apply Hin.
+  inversion Heqb_ident.
 Defined.
+
+
+
+Lemma normalize_type_equation : forall env t,
+    normalize_type env t =
+    match t with
+  | TYPE_Array sz t =>
+    let nt := normalize_type env t in
+    TYPE_Array sz nt
+
+  | TYPE_Function ret args =>
+    let nret := (normalize_type env ret) in
+    let nargs := map_In args (fun t _ => normalize_type env t) in
+    TYPE_Function nret nargs
+
+  | TYPE_Struct fields =>
+    let nfields := map_In fields (fun t _ => normalize_type env t) in
+    TYPE_Struct nfields
+
+  | TYPE_Packed_struct fields =>
+    let nfields := map_In fields (fun t _ => normalize_type env t) in
+    TYPE_Packed_struct nfields
+
+  | TYPE_Vector sz t =>
+    let nt := normalize_type env t in
+    TYPE_Vector sz nt
+
+  | TYPE_Identified id =>
+    let opt := find (fun a => Ident.eq_dec id (fst a)) env in
+    match opt with
+    | None => TYPE_Identified id   (* TODO: should this be None? *)
+    | Some (_, t) => normalize_type (remove_key Ident.eq_dec id env) t
+    end
+
+  | TYPE_I sz => TYPE_I sz
+  | TYPE_Pointer t' => TYPE_Pointer t'
+  | TYPE_Void => TYPE_Void
+  | TYPE_Half => TYPE_Half
+  | TYPE_Float => TYPE_Float
+  | TYPE_Double => TYPE_Double
+  | TYPE_X86_fp80 => TYPE_X86_fp80
+  | TYPE_Fp128 => TYPE_Fp128
+  | TYPE_Ppc_fp128 => TYPE_Ppc_fp128
+  | TYPE_Metadata => TYPE_Metadata
+  | TYPE_X86_mmx => TYPE_X86_mmx
+  | TYPE_Opaque => TYPE_Opaque
+  end.
+Proof.
+  intros env t.
+  unfold normalize_type. 
+  unfold normalize_type_func at 1.
+  rewrite Wf.WfExtensionality.fix_sub_eq_ext.
+  destruct t; try reflexivity. simpl.
+  destruct (find (fun a : ident * typ => Ident.eq_dec id (fst a)) env).
+  destruct p; simpl; eauto.
+  reflexivity.
+Defined.    
+
+
+Hint Constructors unrolled_typ.
+
+
+Lemma find_in_wf_env :
+  forall env id t,
+    NoDup (map fst env) ->
+    In (id, t) env ->
+    find (fun a : ident * typ => Ident.eq_dec id (fst a)) env = Some (id, t).
+Proof.
+  intros env id t Hdup Hin.
+  induction env as [| [id' t'] env].
+  - contradiction.
+  - destruct Hin as [Hin | Hin]; try inversion Hin; subst.
+    + simpl. destruct (Ident.eq_dec id id); intuition.
+    + simpl. destruct (Ident.eq_dec id id').
+      * inversion Hdup. subst. apply in_map with (f:=fst) in Hin. simpl in *.
+        contradiction.
+      * simpl. inversion Hdup.
+        apply IHenv; auto.
+Qed.
+
+
+Lemma guarded_typ_id_same :
+  forall env id,
+    guarded_typ id env (TYPE_Identified id) -> False.
+Proof.
+  intros env id H.
+  inversion H; contradiction.
+Qed.
+
+
+Lemma find_different_key_from_removed :
+  forall env id id',
+    id <> id' ->
+    find (fun a : ident * typ => Ident.eq_dec id' (fst a)) env = find (fun a : ident * typ => Ident.eq_dec id' (fst a)) (remove_key Ident.eq_dec id env).
+Proof.
+  intros env id id' H.
+  induction env.
+  - reflexivity.
+  - destruct a as [i t]. simpl.
+    destruct (Ident.eq_dec id' i) eqn:Heq.
+    + simpl. destruct (Ident.eq_dec id i); subst.
+      * contradiction.
+      * simpl. destruct (Ident.eq_dec i i); try contradiction.
+        reflexivity.
+    + simpl. destruct (Ident.eq_dec id i); subst.
+      * intuition.
+      * simpl. rewrite Heq. simpl. auto.
+Qed.
+
+
+Lemma remove_keys_find :
+  forall env id ids,
+    ~ In id ids ->
+    find (fun a : ident * typ => Ident.eq_dec id (fst a)) env = find (fun a : ident * typ => Ident.eq_dec id (fst a)) (remove_keys Ident.eq_dec ids env).
+Proof.
+  intros env id ids H.
+  induction ids.
+  - reflexivity.
+  - rewrite <- remove_key_keys.
+    rewrite <- find_different_key_from_removed with (id:=a); intuition; subst; intuition.
+Qed.
+
+Lemma trans :
+  forall {A} {a b c : A},
+    c = a ->
+    c = b ->
+    a = b.
+Proof.
+  intros A a b c Hca Hcb.
+  subst. reflexivity.
+Qed.
+
+
+Lemma find_some_id :
+  forall env id p t,
+    NoDup (map fst env) ->
+    In (id, t) env ->
+    find (fun a : ident * typ => Ident.eq_dec id (fst a)) env = Some p ->
+    find (fun a : ident * typ => Ident.eq_dec id (fst a)) env = Some (id, t).
+Proof.
+  intros env id p t Hdup Hin H.
+  induction env.
+  - inversion H.
+  - destruct a. simpl.
+    destruct (Ident.eq_dec id i).
+    + simpl. subst. simpl in Hdup. inversion Hin.
+      * inversion H0. reflexivity.
+      * inversion Hdup. subst.
+        exfalso. apply H3.
+        assert (i = fst (i, t)) by reflexivity.
+        rewrite H1.
+        apply in_map. auto.
+    + simpl. apply IHenv.
+      * simpl in Hdup. inversion Hdup. auto.
+      * simpl in Hin. inversion Hin.
+        -- inversion H0. symmetry in H2. contradiction.
+        -- assumption.
+      * simpl in H. destruct (Ident.eq_dec id i); try contradiction. simpl in H.
+        assumption.
+Qed.
+
+Hint Constructors sized_typ.
+Hint Constructors guarded_typ.
+
+
+(* Types with no identifiers *)
+Inductive simple_typ : typ -> Prop :=
+| simple_typ_I : forall sz, simple_typ (TYPE_I sz)
+| simple_typ_Pointer : forall t, simple_typ t -> simple_typ (TYPE_Pointer t)
+| simple_typ_Void : simple_typ (TYPE_Void)
+| simple_typ_Half : simple_typ (TYPE_Half)
+| simple_typ_Float : simple_typ (TYPE_Float)
+| simple_typ_Double : simple_typ (TYPE_Double)
+| simple_typ_X86_fp80 : simple_typ (TYPE_X86_fp80)
+| simple_typ_Fp128 : simple_typ (TYPE_Fp128)
+| simple_typ_Ppc_fp128 : simple_typ (TYPE_Ppc_fp128)
+| simple_typ_Metadata : simple_typ (TYPE_Metadata)
+| simple_typ_X86_mmx : simple_typ (TYPE_X86_mmx)
+| simple_typ_Array : forall sz t, simple_typ t -> simple_typ (TYPE_Array sz t)
+| simple_typ_Function :
+    forall ret args,
+      simple_typ ret ->
+      (forall a, In a args -> simple_typ a) ->
+      simple_typ (TYPE_Function ret args)
+| simple_typ_Struct :
+    forall fields,
+      (forall f, In f fields -> simple_typ f) ->
+      simple_typ (TYPE_Struct fields)
+| simple_typ_Packed_struct :
+    forall fields,
+      (forall f, In f fields -> simple_typ f) ->
+      simple_typ (TYPE_Packed_struct fields)
+| simple_typ_Opaque : simple_typ (TYPE_Opaque)
+| simple_typ_Vector : forall sz t, simple_typ t -> simple_typ (TYPE_Vector sz t)
+.
+
+
+Hint Constructors simple_typ.
+
+
+Theorem map_in_id :
+  forall {A : Type} (l : list A) (f : forall x : A, In x l -> A),
+    (forall a (Hin : In a l), f a Hin = a) ->
+    map_In l f = l.
+Proof.
+  intros A l f H.
+  induction l; auto.
+  simpl. rewrite H. rewrite IHl; auto.
+Qed.
+
+
+Theorem simple_normalizes_to_self :
+  forall env t,
+    simple_typ t ->
+    normalize_type env t = t.
+Proof.
+  intros env t H.
+  induction H; rewrite normalize_type_equation; simpl;
+    repeat
+      match goal with
+      | [H : normalize_type env _ = _ |- context[normalize_type _ _]] => rewrite H
+      | [|- context[(map_In _ (fun (t : typ) (_ : In t _) => normalize_type env t))]] => rewrite map_in_id; auto
+      end; auto.
+Qed.
+
+
+Theorem simple_unrolled :
+  forall t,
+    simple_typ t -> unrolled_typ t.
+Proof.
+  intros t H.
+  induction H; constructor;
+    try match goal with
+        | [|- Forall _ _] => apply Forall_forall
+        end; auto.
+Qed.
+
+
+Theorem in_map_in :
+  forall {A : Type} (x : A) (l : list A) f,
+    In x (map_In l (fun t (_ : In t l) => f t)) ->
+    exists t, In t l /\ f t = x.
+Proof.
+  intros A x l f H.
+  induction l.
+  - inversion H.
+  - simpl in *. destruct H.
+    + exists a. split; auto.
+    + apply IHl in H as [t [Hin Hftx]].
+      exists t. intuition.      
+Qed.
+
+
+Theorem map_rewrite :
+  forall {A B : Type} (x : A) (l : list A) (f g : A -> B),
+    (forall x, In x l -> f x = g x) ->
+    map_In l (fun t (_ : In t l) => f t) = map_In l (fun t (_ : In t l) => g t).
+Proof.
+  intros A B x l f g H.
+  induction l as [| a l]; simpl; auto.
+  pose proof (H a) as Ha.
+  rewrite Ha; intuition.
+  rewrite IHl; intuition.
+Qed.
+
+
+Theorem guarded_id_normalize_same :
+  forall t env,
+    NoDup (map fst env) ->
+    guarded_wf_typ env t ->
+    (forall ids,
+        (forall id, In id ids -> guarded_typ id env t) ->
+        normalize_type (remove_keys Ident.eq_dec ids env) t = normalize_type env t).
+Proof.
+  intros t env Hdup Hwf.
+  induction Hwf; intros ids Hguard;
+    rewrite normalize_type_equation; symmetry; rewrite normalize_type_equation; simpl; auto.
+  4: { simpl. 
+
+       replace (remove_key Ident.eq_dec id (remove_keys Ident.eq_dec ids defs)) with
+           (remove_keys Ident.eq_dec (id :: ids) defs) by auto using remove_key_keys.
+
+       (* True because id not in ids.
+
+          because if id is in ids, this means that guarded_typ id defs
+          (TYPE_Identified id), which is a contradiction.
+
+        *)
+       assert ((find (fun a : ident * typ => Ident.eq_dec id (fst a)) (remove_keys Ident.eq_dec ids defs)) = (find (fun a : ident * typ => Ident.eq_dec id (fst a)) defs)) as Hfind_removekeys.
+       assert (~ In id ids). unfold not. intros Hinidids.
+       pose proof Hguard id Hinidids as Hguard'.
+       inversion Hguard'; contradiction.
+       symmetry; auto using remove_keys_find.
+
+       rewrite Hfind_removekeys.
+
+       destruct (find (fun a : ident * typ => Ident.eq_dec id (fst a)) defs) eqn:Hfind.
+       - destruct p. simpl.
+
+         assert (In (id, t) defs).
+         apply find_some in Hfind as [Hin Hfind].
+         simpl in Hfind.
+         destruct (Ident.eq_dec id i) eqn:Hidi; subst; intuition.
+         
+         replace (remove_keys Ident.eq_dec ids (remove_key Ident.eq_dec id defs)) with
+             (remove_keys Ident.eq_dec (id :: ids) defs) by auto using remove_keys_key.
+
+         rewrite H2; auto.
+
+         replace (remove_key Ident.eq_dec id defs) with
+             (remove_keys Ident.eq_dec [id] defs) by auto.
+
+         rewrite H2; auto.
+         + intros id0 H4. destruct H4.
+           * subst; auto.
+           * inversion H4.
+         + intros id0 H4. destruct H4.
+           * subst; auto.
+           * pose proof (Hguard id0 H4) as Hguard'. inversion Hguard'; subst.
+             -- rewrite Hfind in H7. inversion H7. subst. auto.
+             -- rewrite Hfind in H9. inversion H9.
+       - reflexivity.
+     }
+  - rewrite IHHwf; auto.
+    rewrite map_rewrite with (f:=normalize_type (remove_keys _ _ _)) (g:=normalize_type defs); auto.
+    intros x H3. apply H2; auto.
+    all: intros id Hidin; pose proof Hguard id Hidin as Hguard'; inversion Hguard'; auto.
+  - rewrite IHHwf; auto.
+    intros id Hidin.
+    pose proof Hguard id Hidin as Hguard'. inversion Hguard'; auto.
+  - rewrite IHHwf; auto;
+    intros id Hidin;
+    match goal with
+    | [H : element_typ _ |- _] => inversion H
+    end; auto.
+  - rewrite map_rewrite with (f:=normalize_type (remove_keys _ _ _)) (g:=normalize_type defs); auto.
+    exact (TYPE_Void).
+    intros x H2. apply H1; auto.
+    intros id Hidin; pose proof Hguard id Hidin as Hguard'; inversion Hguard'; auto.
+  - rewrite map_rewrite with (f:=normalize_type (remove_keys _ _ _)) (g:=normalize_type defs); auto.
+    exact (TYPE_Void).
+    intros x H2. apply H1; auto.
+    intros id Hidin; pose proof Hguard id Hidin as Hguard'; inversion Hguard'; auto.
+Qed.
+
+
+Theorem double_map_In :
+  forall A B C (l : list A) (f : A -> B) (g : B -> C),
+    (map_In (map_In l (fun x (_ : In x l) => f x)) (fun x (_ : In x (map_In l (fun x (_ : In x l) => f x))) => g x)) = map_In l (fun x (_ : In x l) => g (f x)).
+Proof.
+  intros A B C l f g.
+  induction l.
+  - reflexivity.
+  - simpl. auto using f_equal.
+Qed.
+
+
+Theorem guarded_normalize_same :
+  forall t env,
+    NoDup (map fst env) ->
+    guarded_wf_typ env t ->
+    (forall ids,
+        (forall id, In id ids -> guarded_typ id env t) ->
+        normalize_type env (normalize_type env t) = normalize_type env t).
+Proof.
+  intros t env Hdup Hwf ids Hguard_all.
+  induction Hwf; try solve [rewrite normalize_type_equation; symmetry; rewrite normalize_type_equation; simpl; auto].
+  - rewrite normalize_type_equation; symmetry; rewrite normalize_type_equation; simpl; auto.
+
+    rewrite IHHwf; auto.
+    rewrite double_map_In.
+    rewrite map_rewrite with (f:=fun x => normalize_type defs (normalize_type defs x)) (g:=normalize_type defs); auto.
+    intros x Hin. apply H2; auto.
+    all: intros id Hinids; pose proof Hguard_all _ Hinids as Hguard'; inversion Hguard'; auto.
+
+  - rewrite normalize_type_equation; symmetry; rewrite normalize_type_equation; simpl; auto.
+
+    rewrite IHHwf; auto.
+    intros id Hinids; pose proof Hguard_all _ Hinids as Hguard'; inversion Hguard'; auto.
+
+  - rewrite normalize_type_equation; symmetry; rewrite normalize_type_equation; simpl; auto.
+
+    rewrite IHHwf; auto.
+    intros id Hinids;
+      match goal with
+      | [H : element_typ _ |- _] => inversion H
+      end; auto.
+  - symmetry. rewrite normalize_type_equation. simpl.
+
+    destruct (find (fun a : ident * typ => Ident.eq_dec id (fst a)) defs) eqn:Hfind.
+    + destruct p.
+
+      assert (In (id, t) defs).
+      apply find_some in Hfind as [Hin Hfind].
+      simpl in Hfind.
+      destruct (Ident.eq_dec id i) eqn:Hidi; subst; intuition.
+
+      symmetry.
+      replace (remove_key Ident.eq_dec id defs) with (remove_keys Ident.eq_dec [id] defs) by auto.
+      rewrite guarded_id_normalize_same; auto.
+      apply H2; auto.
+      * intros id0 Hinids; pose proof Hguard_all _ Hinids as Hguard'. inversion Hguard'; auto; subst.
+        -- rewrite Hfind in H6. inversion H6; subst; auto.
+        -- rewrite Hfind in H8. inversion H8.
+      * intros id0 H4. inversion H4. subst. auto.
+        inversion H5.
+    + rewrite normalize_type_equation. simpl. rewrite Hfind. reflexivity.
+  - rewrite normalize_type_equation; symmetry; rewrite normalize_type_equation; simpl; auto.
+    rewrite double_map_In.
+    rewrite map_rewrite with (f:=fun x => normalize_type defs (normalize_type defs x)) (g:=normalize_type defs); auto.
+    exact TYPE_Void.
+    intros x H2. rewrite H1; auto.
+    intros id0 Hinids; pose proof Hguard_all _ Hinids as Hguard'. inversion Hguard'; auto.
+  - rewrite normalize_type_equation; symmetry; rewrite normalize_type_equation; simpl; auto.
+    rewrite double_map_In.
+    rewrite map_rewrite with (f:=fun x => normalize_type defs (normalize_type defs x)) (g:=normalize_type defs); auto.
+    exact TYPE_Void.
+    intros x H2. rewrite H1; auto.
+    intros id0 Hinids; pose proof Hguard_all _ Hinids as Hguard'. inversion Hguard'; auto.
+Qed.
+
+
+Lemma wf_typ_guarded_normalize_twice :
+  forall env t,
+    NoDup (map fst env) ->
+    wf_typ env t ->
+    (forall ids,
+        (forall id, In id ids -> guarded_typ id env t) ->
+        normalize_type env (normalize_type env t) = normalize_type env t).
+Proof.
+  eauto using wf_typ_is_guarded_wf_typ, guarded_normalize_same.
+Qed.
+
+
+Theorem double_normalize_type :
+  forall env t,
+    wf_env env ->
+    wf_typ env t ->
+    normalize_type env (normalize_type env t) = normalize_type env t.
+Proof.
+  intros env t [Hdup Henv] Hwf.
+  induction Hwf; try solve [rewrite normalize_type_equation; symmetry; rewrite normalize_type_equation; simpl; auto].
+  4 : {
+        simpl.
+
+        symmetry.
+        rewrite normalize_type_equation. simpl.
+
+        destruct (find (fun a : ident * typ => Ident.eq_dec id (fst a)) defs) as [[i t] |] eqn:Hfind.
+        - 
+          apply find_some in Hfind as [Hin Heq].
+          simpl in *. destruct (Ident.eq_dec id i); inversion Heq; subst.
+
+          replace (remove_key _ i defs) with (remove_keys Ident.eq_dec [i] defs) by auto.
+
+
+          rewrite guarded_id_normalize_same; auto using wf_typ_is_guarded_wf_typ.
+          + symmetry. apply H2; auto.
+          + intros id H3.
+            inversion H3; subst; try contradiction; auto.
+        - rewrite normalize_type_equation. simpl. rewrite Hfind.
+          reflexivity.
+        }
+
+        - rewrite normalize_type_equation. symmetry. rewrite normalize_type_equation.
+          simpl. rewrite double_map_In.
+          rewrite IHHwf; auto.
+          symmetry.
+          rewrite map_rewrite with (g:=normalize_type defs) at 1; auto.
+        - rewrite normalize_type_equation. symmetry. rewrite normalize_type_equation.
+          simpl. rewrite IHHwf; auto.
+        - rewrite normalize_type_equation. symmetry. rewrite normalize_type_equation.
+          simpl. rewrite IHHwf; auto.
+        - rewrite normalize_type_equation. symmetry. rewrite normalize_type_equation.
+          simpl. rewrite double_map_In.
+          symmetry.
+          rewrite map_rewrite with (g:=normalize_type defs) at 1; auto.
+          exact TYPE_Void.
+        - rewrite normalize_type_equation. symmetry. rewrite normalize_type_equation.
+          simpl. rewrite double_map_In.
+          symmetry.
+          rewrite map_rewrite with (g:=normalize_type defs) at 1; auto.
+          exact TYPE_Void.
+Qed.
+
+
+(*
+Theorem normalize_type_unrolls:
+  forall et : list (ident * typ) * typ,
+    wf_env (fst et) ->
+    wf_typ (fst et) (snd et) ->
+    unrolled_typ (normalize_type (fst et) (snd et)).
+Proof.
+  TODO
+Qed.
+*)
